Lampe/Lampe/Builtin/Slice.lean
@@ -60,7 +60,7 @@ where `l'` is `l` except that `e` is inserted at index `i`, and all the elements
 In Noir, this builtin corresponds to `fn insert(self, index: u32, elem: T) -> Self` implemented for `[T]`.
 -/
 def sliceInsert := newGenericPureBuiltin
-  (fun tp => ⟨[.slice tp, .i 32, tp], .slice tp⟩)
+  (fun tp => ⟨[.slice tp, .u 32, tp], .slice tp⟩)
   (fun _ h![l, i, e] => ⟨i.toNat < l.length,
     fun _ => l.insertNth i.toNat e⟩)
 
@@ -87,7 +87,7 @@ We make the following assumptions:
 In Noir, this builtin corresponds to `fn pop_back(self) -> (Self, T)` implemented for `[T]`.
 -/
 def slicePopBack := newGenericPureBuiltin
-  (fun tp => ⟨[Tp.slice tp], Tp.struct [Tp.slice tp, tp]⟩)
+  (fun tp => ⟨[.slice tp], .struct [.slice tp, tp]⟩)
   (fun _ h![l] => ⟨l ≠ [],
     fun h => (l.dropLast, l.getLast h, ())⟩)
 
@@ -101,7 +101,7 @@ where `l'` is `l` except that the element at index `i` is removed, and all the e
 In Noir, this builtin corresponds to `fn remove(self, index: u32) -> (Self, T)` implemented for `[T]`.
 -/
 def sliceRemove := newGenericPureBuiltin
-  (fun tp => ⟨[.slice tp, Tp.i 32], .struct [.slice tp, tp]⟩)
+  (fun tp => ⟨[.slice tp, .u 32], .struct [.slice tp, tp]⟩)
   (fun _ h![l, i] => ⟨i.toNat < l.length,
     fun h => (l.eraseIdx i.toNat, l.get (Fin.mk i.toNat h), ())⟩)
 
