Lampe/Lampe/Hoare/Builtin/Cmp.lean
@@ -1,0 +1,20 @@
+import Lampe.Ast
+import Lampe.Tp
+import Lampe.Semantics
+import Lampe.SeparationLogic
+import Lampe.Hoare.Total
+import Lampe.Hoare.SepTotal
+
+namespace Lampe.STHoare
+
+theorem eq_intro {tp} {a b : tp.denote p} :
+  STHoare p Γ
+      ⟦⟧
+      (.call h![] [tp, tp] .bool (.builtin .eq) h![a, b])
+      (fun v => ∃h, v = ((Builtin.tpBEq tp).get h).beq a b) := by
+  apply pureBuiltin_intro_consequence <;> try tauto
+  intro h
+  simp only
+  simp_all only [exists_const]
+
+end Lampe.STHoare
